# Finding a function

You can find the function by simply replacing `x` with the given expression and then working out the new function.

## Example

```Math
f(x) = 2x^3 + 4
Let f(7)

Replace x with the new expression
f(7) = 2(7)^3 + 4

Using BODMAS, work out the expression
f(7) = 2(343) + 4    // 7 times 7 times 7
f(7) = 686 + 4    // 2 times 343
f(7) = 690    // Added the 4

Since no more calculations or simplifcations can be done. That's it.
```

```Math
f(x) = 2x^3 + 4
let f(-0.5)

Replace x with the new expression
f(-0.5) = 2(-0.5)^3 + 4

Using BODMAS, work out the expression
f(-0.5) = 2(-0.125) + 4    // -0.5 times -0.5 times -0.5
f(0.5) = -0.25 + 4    // -0.125 times 2
f(-0.5) = 3.75    // -0.25 add 4

Since no more calculations or simplifcations can be done. That's it.
```

# Finding funtion of function

To find a function of another function, you have to replace `x` by the other function of the order. For example `g` of `f`; in this situation `f` goes where the `x` would be in the function of `g`.

## Examples

```Math
f(x) = 4x + 2
g(x) = x + 3

In this case, multiplying g with f is easier
g(x) = x + 3
Would be
g(4x+2) = (4x + 2) + 3

Using BODMAS nothing can be done in the brackets so they are removed
4x + 2 + 3

Simply the equation by adding together items
4x + 5

Since nothing else can be done, that's it.
```

# Corresponding expression

This is simplifying the expression down. To do this we replace `x` with the expression given and then work out the new expression.

## Example

```Math
f(4x + 2) âˆ’ f(x) when f(x) = x^2

Replace the x with our newly given expression
f(4x + 2)^2 - f
(x)^2

Now we work out the equation using BODMAS
(4x + 2)^2 = (4x + 2) times (4x + 2) = 16x^2 + 8x + 8x + 4
	4x times 4x = 16x^2
	4x times 2 = 8x
	4x times 2 = 8x
	2 times 2 = 4

x^2 = x times x = x^2

Putting these together using the original equation
16x^2 + 8x + 8x - x^2

Simply it
	16x^2 - x^2 = 15x^2
15x^2 + 16x + 4
```

# Inverse

To do an inverse, you have to make x the sole remaining part of the right-side of the equation.

You do this by replacing the function with `Y`.

Then you remove numbers from the side with `X`. By doing this you must also do the same to the other side.

Then you put the equation of `f-1` in by replacing `Y` with `X`

## Examples

```Math
f(x) = 7 + 5x

Replace f(x) with Y
Y = 7 + 5x

Using BODMAS, remove numbers from the right side to the left side
Y-7 = 5x    // Minus 7 from both sides
(Y-7)/5 = x    // Divide by 5

Now that x is alone we use f-1
f-1(x) = (x-7)/5
```

```Math
f(x) = 3x

Replace f(x) with Y
Y = 3x

Using BODMAS, remove numbers from the right side to the left side
Y/3 = x    // Divide by 3

Now that x is alone we use f-1
f-1(x) = x/3
```